Consider a constant force \(\vec F\) causing a ball of mass \(m\) which is moving at a velocity \(\vec v\) to come to rest over a distance \(\vec s\).

TODO\@: TikZ diagram

Using SUVAT\@:

\begin{equation}
  v^2 = u^2 + 2as
\end{equation}

But since it comes to rest, \(v = 0\), and the initial velocity \(u = \abs{\vec v}\). Rearranging for \(a\):

\begin{align}\label{eq:proof-ke-as}
  0 &= v^2 + 2as \notag \\
  v^2 &= -2as \notag \\
  -\frac{v^2}{2} &= as \notag \\
  as &= -\frac{v^2}{2}
\end{align}

Since the work done \(W\) by a constant force is given by:

\begin{equation}
  W = \vec F \cdot \vec s = m \vec a \cdot \vec s
\end{equation}

We can substitute equation~\ref{eq:proof-ke-as} into this to get something already resembling the kinetic energy formula:

\[
  \begin{aligned}
    W &= m \cdot -\frac{v^2}{2} \\
    W &= -\frac 1 2 mv^2
  \end{aligned}
\]

Since the work done \(W\) is equal to the change in kinetic energy, and the particle ends at rest, we have:

\[
  \begin{aligned}
    W &= E_{kf} - E_{ki} \\
    W &= 0 - E_{ki} \\
    W &= -E_{ki} \\
    E_{ki} &= -W \\
    E_{ki} &= \frac 1 2 mv^2
  \end{aligned}
\]
